WIP

src/lib/Red2.v
@@ -1,26 +1,4 @@
-From Ltac2 Require Import Ltac2.
-From Ltac2 Require Option Array Ident Control Std Fresh Message.
-
-Ltac2 or t0 t1 :=
-  match! 'True with
-  | True => t0 ()
-  | _ => t1 ()
-  end.
-
-Ltac2 fail () := Control.zero Match_failure.
-
-Ltac2 tcsearch e :=
-  let x := Array.make 1 constr:(tt: unit) in
-  or (fun _ =>
-        let n := Fresh.in_goal ident:(_TC_) in
-        ltac1:(e n|- unshelve evar (n: e);
-               [typeclasses eauto|]) (Ltac1.of_constr e) (Ltac1.of_ident n);
-        Array.set x 0 (Std.eval_unfold [(Std.VarRef n, Std.AllOccurrences)] (Control.hyp n));
-        fail ())
-     (fun _ => Array.get x 0)
-.
-
-Set Default Proof Mode "Classic".
+From Fairness Require Import MyLtac2.
 
 Ltac2 Type flag := [ Break | Continue | Fail ].
 
@@ -31,7 +9,7 @@ Lemma _equal_f (A B : Type) (f g : A -> B)
   :
     f x = g x.
 Proof.
-  subst. apply eq_refl.
+  subst. apply (@eq_refl).
 Qed.
 
 Lemma _einit (P Q: Prop)
@@ -43,64 +21,289 @@ Proof.
 Qed.
 
 Ltac2 rec _ctx n :=
-  match! n with
-  | O => apply f_equal
-  | S ?m => apply _equal_f; _ctx m
-  end.
-
-Ltac2 __prw red_tac success :=
-  cbn;
-  tryif (let f := fresh "f" in
-         evar (f:_flag);
-         etransitivity;
-         [red_tac|
-           match goal with
-           | [f0:= ?f1: _flag|- _] =>
-               match f1 with
-               | _continue => subst f; __prw red_tac true
-               | _break => subst f; reflexivity
-               | _fail => fail 2
-               end
-           end])
+  if (Int.le n 0)
   then
-    idtac
+    (apply f_equal)
   else
-    match success with
-    | true => reflexivity
-    | false => fail
-    end.
+    (apply _equal_f; _ctx (Int.sub n 1))
+.
 
-Ltac _prw k0 k1 X :=
+(* Ltac2 __prw red_tac success := *)
+(*   cbn; *)
+(*   tryif (let f := fresh "f" in *)
+(*          evar (f:_flag); *)
+(*          etransitivity; *)
+(*          [red_tac| *)
+(*            match goal with *)
+(*            | [f0:= ?f1: _flag|- _] => *)
+(*                match f1 with *)
+(*                | _continue => subst f; __prw red_tac true *)
+(*                | _break => subst f; reflexivity *)
+(*                | _fail => fail 2 *)
+(*                end *)
+(*            end]) *)
+(*   then *)
+(*     idtac *)
+(*   else *)
+(*     match success with *)
+(*     | true => reflexivity *)
+(*     | false => fail *)
+(*     end. *)
+
+Class Foo (n: nat) := mk_Foo {}.
+Instance foo: Foo 3 := mk_Foo _.
+
+Import Constr.Binder Constr.Unsafe.
+
+
+
+From Ltac2 Require Export Ltac2.
+
+Goal forall X Y (f: X -> Y) (x: X) (y: Y), f x = y.
+Proof.
+  intros.
+  let d := open_constr:(fun _t => _ _t = _) in
+  let c := Std.eval_hnf open_constr:($d _) in
+  Std.unify c (Control.goal ());
+  Std.pose None d;
+  let c := open_constr:(@eq_rect_r X _ $d) in
+  eapply $c.
+
+
+ _ _ _)
+  .
+
+
+  let u := open_constr:(_: ltac:(exact_no_check $t)) in
+  match Constr.Unsafe.kind u with
+  | Constr.Unsafe.Cast v _ _ =>
+      let f := open_constr:(fun _t => _ _t = _) in
+      Std.unify open_constr:($f _) (Control.goal ());
+      Std.pose None f
+      v
+  | _ => Control.throw Init.Assertion_failure
+  end
+  .
+
+
+  .
+
+
+  let n := Fresh.in_goal ident:(x) in
+  let b := Constr.Binder.make (Some n) open_constr:(X) in
+  let x := Constr.Unsafe.make (Constr.Unsafe.Rel 1) in
+  let a := Constr.Unsafe.make (Constr.Unsafe.Lambda b open_constr:(_ $x = _)) in
+  Std.unify constr:($a x) (Control.goal ());
+  Std.pose None a
+  .
+
+  end.
+
+ =>
+                                 match (Constr.Unsafe.kind c) with
+                                 | Rel n
+                                   => Message.print (Message.of_int n)
+
+
+open_constr:(fun _t => _ _t = _) in
+  Std.unify constr:($a x) (Control.goal ());
+  Std.pose None a
+  .
+
+
+  match (Constr.Unsafe.kind constr:(fun x: nat => x)) with
+  | Constr.Unsafe.Lambda b c =>
+      match (Constr.Unsafe.kind c) with
+      | Rel n
+        => Message.print (Message.of_int n)
+
+
+
+
+    (* | Var _ *)
+      (*   => Message.print (Message.of_string "1") *)
+      (* | Meta _ *)
+      (*   => Message.print (Message.of_string "2") *)
+      (* | Evar _ _ *)
+      (*   => Message.print (Message.of_string "3") *)
+      (* | Sort _ *)
+      (*   => Message.print (Message.of_string "4") *)
+      (* | Cast _ _ _ *)
+      (*   => Message.print (Message.of_string "5") *)
+      (* | Prod _ _ *)
+      (*   => Message.print (Message.of_string "6") *)
+      (* | Lambda _ _ *)
+      (*   => Message.print (Message.of_string "7") *)
+      (* | LetIn _ _ _ *)
+      (*   => Message.print (Message.of_string "8") *)
+      (* | App _ _ *)
+      (*   => Message.print (Message.of_string "9") *)
+      (* | Constant _ _ *)
+      (*   => Message.print (Message.of_string "10") *)
+      (* | Ind _ _ *)
+      (*   => Message.print (Message.of_string "11") *)
+      (* | Constructor _ _ *)
+      (*   => Message.print (Message.of_string "12") *)
+      (* | Case _ _ _ _ _ *)
+      (*   => Message.print (Message.of_string "13") *)
+      (* | Fix _ _ _ _ *)
+      (*   => Message.print (Message.of_string "14") *)
+      (* | CoFix _ _ _ *)
+      (*   => Message.print (Message.of_string "15") *)
+      (* | Proj _ _ *)
+      (*   => Message.print (Message.of_string "16") *)
+      (* | Uint63 _ *)
+      (*   => Message.print (Message.of_string "17") *)
+      (* | Float _ *)
+      (*   => Message.print (Message.of_string "18") *)
+      (* | Array _ _ _ _ *)
+      (*   => Message.print (Message.of_string "19") *)
+      | _ => Control.throw Init.Assertion_failure
+      end
+  | _ => Control.throw Init.Assertion_failure
+  end
+  .
+
+
+Some c =>
+      let c := Constr.Unsafe.make (Constr.Unsafe.Var c) in
+      let a := Constr.Unsafe.make (Constr.Unsafe.Lambda b open_constr:(_ $c = _)) in
+      Std.unify constr:($a x) (Control.goal ());
+      Std.pose None a
+  | _ => Control.throw Init.Assertion_failure
+  end
+  .
+
+
+
+
+  let n := Fresh.in_goal ident:(_TC_) in
+  let b := Constr.Binder.make (Some n) constr:(X) in
+  match (Constr.Binder.name b) with
+  | Some c =>
+      let c := Constr.Unsafe.make (Constr.Unsafe.Var c) in
+      let a := Constr.Unsafe.make (Constr.Unsafe.Lambda b open_constr:(_ $c = _)) in
+      Std.unify constr:($a x) (Control.goal ());
+      Std.pose None a
+  | _ => Control.throw Init.Assertion_failure
+  end
+  .
+
+  let a := open_constr:(fun _t => _ _t = _) in
+  Std.unify constr:($a x) (Control.goal ());
+  Std.pose None a
+  .
+
+
+  let n := Fresh.in_goal ident:(_TC_) in
+  let b := Constr.Binder.make (Some n) constr:(X) in
+  match (Constr.Binder.name b) with
+  | Some c =>
+      let c := Constr.Unsafe.make (Constr.Unsafe.Var c) in
+      let a := Constr.Unsafe.make (Constr.Unsafe.Lambda b open_constr:(_ $b = _)) in
+      Std.unify constr:($a x) (Control.goal ());
+      Std.pose None a
+  | _ => Control.throw Init.Assertion_failure
+  end
+  .
+
+
+ ().
+
+
+  let n := Fresh.in_goal ident:(_TC_) in
+  let a := open_constr:(fun $n => _ $n = _) in
+  Std.unify constr:($a x) (Control.goal ());
+  Std.pose None a
+  .
+  Show Proof.
+
+  let n := Fresh.in_goal ident:(_TC_) in
+  Std.in_context
+
+
+
+Goal False.
+Proof.
+  assert (Foo 3).
+  { pose foo.
+
+let n := Fresh.in_goal ident:(_TC_) in
+    let m := (Constr.in_context n constr:(unit) (fun _ => typeclasses_eauto)) in
+    Message.print (Message.of_constr m).
+
+
+Message.print (mes.
+
+
+
+
+Ltac2 @ external in_context : ident -> constr -> (unit -> unit) -> constr := "coq-core.plugins.ltac2" "constr_in_context".
+(** On a focused goal [Γ ⊢ A], [in_context id c tac] evaluates [tac] in a
+    focused goal [Γ, id : c ⊢ ?X] and returns [fun (id : c) => t] where [t] is
+    the proof built by the tactic. *)
+
+  intros.
+  Std.unify
+
+
+Ltac2 rec holes pos :=
+  match pos with
+  | hd::tl =>
+      if (Int.le hd 0)
+      then
+        let k := holes tl in
+        open_constr:($k _)
+      else
+        holes tl
+  | [] =>
+      open_constr:(4)
+  end.
+
+
+
+
+open_constr:(_: ltac:(exact_no_check $t))
+
+                       |
+
+
+  if (Int.le n 0)
+  then
+    (apply f_equal)
+  else
+    (apply _equal_f; _ctx (Int.sub n 1))
+
+
+  match n with
+  |
+
+  match holes with
+  | hd::tl =>
+
+Ltac2 rec holes pos :=
+  match holes with
+  | hd::tl =>
+
+
+Ltac2 evar t n :=
+  let u := open_constr:(_: ltac:(exact_no_check $t)) in
+  match Constr.Unsafe.kind u with
+  | Constr.Unsafe.Cast v _ _ =>
+      Std.pose n t;
+      v
+  | _ => Control.throw Init.Assertion_failure
+  end
+.
+
+Ltac2 _prw k0 k1 X :=
   match X with
-  | O => eapply _einit; [(k0; k1)|]
+  | O => eapply _einit > [(k0; k1)|]
   | S ?n => _prw ltac:(k0; _ctx n) k1
-  end.
-
-Ltac _rwb k X :=
-  match X with
-  | O => k
-  | _ => _rwb ltac:(fun f => ltac:(k f || (instantiate (f:=_break); eapply X; fail)))
-  end.
-
-Ltac _rwc k X :=
-  match X with
-  | O => k
-  | _ => _rwc ltac:(fun f => ltac:(k f || (instantiate (f:=_continue); eapply X; fail)))
-  end.
-
-Ltac _rwa k X :=
-  match X with
-  | O => k
-  | (?H, ?_f) => _rwa ltac:(fun f => ltac:(k f || (instantiate (f:=_f); eapply H; fail)))
   end.
 
 (* Main Tactic *)
 Ltac prw red_tac X := _prw ltac:(idtac) ltac:(__prw red_tac false) X.
-
-Ltac rwbl X := _rwb ltac:(fun f => fail) X.
-Ltac rwcl X := _rwc ltac:(fun f => fail) X.
-Ltac rwal X := _rwa ltac:(fun f => fail) X.
-Ltac rrw X _f := ltac:(fun f => instantiate (f:=_f); eapply X; fail).
 
 Module TUTORIAL.
   Section FOO.
@@ -175,3 +378,5 @@ Module TUTORIAL.
     Qed.
   End FOO.
 End TUTORIAL.
+
+? _
