src/lib/IRed2.v
@@ -1,5 +1,5 @@
 Require Import String Program.
-From Fairness Require Export TRed.
+From Fairness Require Export TRed2.
 From Fairness Require Import ITreeLib Event.
 
 Definition itree_class: red_class := red_class_cons "itree".
@@ -9,7 +9,7 @@ Global Opaque itree_unfold.
 Definition itree_option: red_class := red_class_cons "itree_option".
 Global Opaque itree_option.
 
-#[export] Instance incl_itree_unfold_itree_class: red_db_incl itree_unfold itree_class := mk_red_db_incl.
+#[export] Instance incl_itree_unfold_itree_class: red_db_incl itree_class := mk_red_db_incl _ itree_unfold.
 
 #[export] Instance focus_bind E X Y (itr: itree E X) (ktr: X -> itree E Y)
   : red_db itree_class (itr >>= ktr) :=
